unmangling error

src/tls/IK.fst
@@ -6,11 +6,17 @@ module IK
 /// * captures nested derivations via bounded-recursive instantiation.
 /// * applied to an extract/expand schedule (simplified from TLS 1.3)
 /// * models partial key compromise, controlled by the adversary for each new key
+/// * features agility and ideal-only indexes.
 ///
-/// Not done yet: conditional idealization and erasure; agility. 
+/// Not done yet: conditional idealization and erasure.
 
-type lbytes (len:UInt32.t)
+assume type lbytes (len:UInt32.t)
+assume val sample: len:UInt32.t -> lbytes len  // not pure!
 
+/// How to deal with agility etc? Key (i:id) (u:usage) where u is
+/// concrete, and usually bound to i---in which case it is Ok to
+/// select u at derivation-time.
+ 
 /// --------------------------------------------------------------------------------------------------
 /// We embed first-class modules as datatype "packages"
 ///
@@ -27,27 +33,67 @@ noeq type ipkg = | Idx:
 /// indexes, but concrete on their key randomness; instances may have
 /// any number of other functions (such a leak, for instance).
 noeq type pkg (ip:ipkg) = | Pkg:
-  key: (Idx?.t ip -> Type0) -> 
-  len: (Idx?.t ip -> UInt32.t) ->
-  create: (i:Idx?.t ip -> key i) -> 
-  coerce: (i:Idx?.t ip {~(Idx?.honest ip i)} -> lbytes (len i) -> key i) ->
+  use: Type0 -> 
+  key: (ip.t -> use -> Type0) -> 
+  len: (use -> UInt32.t) ->
+  create: (i:ip.t -> u:use -> key i u) -> 
+  coerce: (i:ip.t {~(ip.honest i)} -> u:use -> lbytes (len u) -> key i u) ->
   pkg ip
+
+/// pick an ordering: ip.t -> use for now.
+///
+/// We must ensure a shared `use` for all instances (or only when
+/// idealized?); this may follow from static memoization.
+/// 
+/// Do we want to hardwire that u is a function of i? 
+
+/// --------------------------------------------------------------------------------------------------
+/// module AEAD
+/// sample agile functionality,
+
+type aeadAlg = | AES_GCM128 | AES_GCM256
+let aeadLen = function
+  | AES_GCM128 -> 32ul
+  | AES_GCM256 -> 48ul
+
+type keyrepr a = lbytes (aeadLen a)
+assume new type key (#ip: ipkg) (i: ip.t) (a:aeadAlg) // abstraction required for indexing
+assume val create_key: #ip: ipkg -> i: ip.t -> a:aeadAlg -> key i a
+assume val coerce_key: #ip: ipkg -> i: ip.t -> a:aeadAlg -> keyrepr a -> key i a
+
+let mp (ip:ipkg): pkg ip = 
+  Pkg aeadAlg key aeadLen create_key coerce_key
+
+val encrypt: #ip:ipkg -> #i:ip.t -> #a:aeadAlg -> k: key i a -> nat -> nat 
+let encrypt #ip #i #a k v = v + 1
+
+/// --------------------------------------------------------------------------------------------------
+/// module Raw
+/// a default functionality (no idealization);
+/// for modelling, we could also provide a "leak" function
+///
+type keylen = n:UInt32.t { UInt32.v n < 128 }
+type raw  (#ip: ipkg) (i: Idx?.t ip) (len:keylen) = lbytes len
+let create_raw (#ip: ipkg) (i: ip.t) (len:keylen): raw  i len = sample len
+let coerce_raw (#ip: ipkg) (i: ip.t) (len:keylen) (r:lbytes len): raw i len = r
+let rp (ip:ipkg): pkg ip = Pkg keylen raw (fun n -> n) create_raw coerce_raw
 
 /// --------------------------------------------------------------------------------------------------
 /// module Index
 
-/// we provide an instance of ipkg to track key derivation (here using constant labels)
+/// We provide an instance of ipkg to track key derivation (here using constant labels)
 type label = string 
-type usage = string -> ip:ipkg -> pkg ip
+
+/// We expect this function to be fully applied at compile time.
+type usage (a:Type0) (ip:ipkg) =  label -> p:pkg ip & (ctx:a -> p.use)
 
 type id_dhe = nat // simplification: instead of the index, use  materials (g,X,Y)
-
 type id_psk = nat // external application PSKs only; we may need a special PSK0 constructor too
 type id = 
   | Zero // symbolic constant for absent extraction arguments
-  | Preshared of id_psk  /// external application PSKs only
+  | Preshared of id_psk  // external application PSKs only
   | Extract0: materials:id -> id
-  | Extract1: salt:id -> materials: id_dhe -> id
+  | Extract1: salt:id -> materials: id_dhe -> id // do we need 2 cases?
   | Extract2: salt:id  -> id
   | Derived: id -> label -> id  
 
@@ -76,7 +122,19 @@ let ii:ipkg = Idx id (fun _ -> true)
 /// we define a KDF parametric in both its usage and ipkg
 /// We rely on type abstraction to separate secrets with different indexes
 /// For soundness, we must also prevent external calls to create derived secrets.
-assume new type secret (u:usage) (ip: ipkg) (i: ip.t)
+type kdfa = | SHA1 | SHA2
+type info = {ha:kdfa; aea:aeadAlg} (* runtime *) 
+//type suse = a:info * usage info ii
+
+let secret_len a = 
+  match a.ha with 
+  | SHA1 -> 8ul
+  | SHA2 -> 16ul 
+assume new type secret 
+  (ip: ipkg) 
+  (u: usage info ip)
+  (i: ip.t) 
+  (a: info) 
 
 /// Real KDF schemes, parameterized by an algorithm computed from the
 /// index (existing code).
@@ -84,46 +142,57 @@ assume new type secret (u:usage) (ip: ipkg) (i: ip.t)
 /// maybe reverse-inline sampling from low-level KeyGen?
 /// otherwise we have to argue it is what Create does.
 
-val create: 
-  u: usage -> 
-  ip: ipkg ->
-  i: ip.t ->
-  secret u ip i
-let create u ip i = admit()
-
 val coerce: 
-  u: usage -> 
   ip: ipkg ->
-  i: Idx?.t ip ->
-  repr: lbytes 32ul -> 
-  secret u ip i
-let coerce u ip i repr = admit()
+  u: usage info ip ->
+  i: ip.t ->
+  a: info (* run-time *) -> 
+  repr: lbytes (secret_len a) -> 
+  secret ip u i a 
+let coerce ip u i a repr = admit()
 
-let pp (u:usage) (ip:ipkg): pkg ip = Pkg 
-  (secret u ip) 
-  (fun _ -> 32ul) 
-  (create u ip) 
-  (coerce u ip)
+val create: 
+  ip: ipkg ->
+  u: usage info ip -> 
+  i: ip.t ->
+  a: info (* run-time *) ->
+  secret ip u i a
+let create ip u i a = 
+  let raw = sample (secret_len a) in
+  coerce ip u i a raw
+
+let pp (ip:ipkg) (u: usage info ip): pkg ip = Pkg 
+  info
+  (secret ip u) 
+  secret_len
+  (create ip u) 
+  (coerce ip u)
 
 /// TODO consider separating pp packages more explicitly, so that we
 /// can idealize them one at a time. (Having one proof step for each
 /// nested level of key derivation seems unavoidable.)
 
-val derive:
-  #u:usage ->
-  #i: id -> 
-  k: secret u ii i ->
-  v: label ->
-  (u v ii).key  (Derived i v)  
+let derived_key (u: usage info ii) (i: id) (v:label) (a: info) = 
+  let (| pkg', derived_alg |) = u v in 
+  pkg'.key (Derived i v) (derived_alg a)
 
-let derive #u #i k v = 
-  let pkg = u v ii in
+val derive:
+  #u: usage info ii ->
+  #i: id ->
+  a: info -> 
+  k: secret ii u i a ->
+  v: label ->
+  derived_key u i v a 
+
+let derive  #u #i a k v = 
+  let (| pkg', derived_alg |) = u v in 
+  let a' = derived_alg a in 
   if ii.honest (*safe*) i // (Derived i v) 
   then
-    pkg.create (Derived i v) //keybytes 
+    pkg'.create (Derived i v) a' //keybytes 
   else 
-    let repr: lbytes (pkg.len (Derived i v)) = admit() in 
-    pkg.coerce (Derived i v) repr
+    let raw = sample (pkg'.len a') in 
+    pkg'.coerce (Derived i v) a' raw
 
 /// Reconsider packaging: should create take external randomness?
 ///
@@ -137,102 +206,100 @@ let derive #u #i k v =
 
 /// covering two cases: application PSK and resumption PSK
 /// (the distinction follow from the value of i)
-type psk (expu: usage) (ip: ipkg) (i: ip.t)
+assume type psk 
+  (#ip: ipkg) 
+  (#u: usage info ip) 
+  (i: ip.t) 
+  (a:info) 
+
+// ip:ipkg or fixed id?
 
 assume val create_psk: 
-  #expu: usage -> 
   #ip: ipkg -> 
+  #u: usage info ip ->
   i: ip.t -> 
-  psk expu ip i 
+  a: info -> 
+  psk #ip #u i a
 
 assume val coerce_psk: 
-  #expu: usage -> 
   #ip: ipkg -> 
+  #u: usage info ip ->
   i: ip.t -> 
-  raw: lbytes 16ul -> 
-  psk expu ip i 
+  a: info -> 
+  raw: lbytes (secret_len a) -> 
+  psk #ip #u i a
 
-let pskp (expu:usage) (ip:ipkg): pkg ip = Pkg 
-  (psk expu ip)
-  (fun _ -> 16ul) 
-  create_psk 
-  coerce_psk
+let pskp (ip:ipkg) (u:usage info ip): pkg ip = Pkg 
+  info 
+  psk
+  secret_len
+  create_psk
+  (coerce_psk #ip #u)
+  
 
 /// Derived salt; note it is already indexed by the usage of the
 /// following extension.
-type salt (expu: usage) (ip:ipkg) (i: ip.t) 
+assume type salt (ip:ipkg) (u: usage info ip) (i: ip.t)  (a: info)
 
 assume val create_salt: 
-  #expu: usage -> 
   #ip: ipkg -> 
+  #u: usage info ip -> 
   i: ip.t -> 
-  salt expu ip i 
+  a: info -> 
+  salt ip u i a
 
 assume val coerce_salt: 
-  #expu: usage ->
   #ip: ipkg ->
+  #u: usage info ip ->
   i: ip.t ->
-  raw: lbytes 16ul ->
-  salt expu ip i 
+  a: info -> 
+  raw: lbytes (secret_len a) ->
+  salt ip u i a
 
-let saltp1 (expu:usage) (ip:ipkg): pkg ip = Pkg 
-  (salt expu ip)
-  (fun _ -> 16ul) 
+// use instances of the same package for both? 
+
+let saltp1 (ip:ipkg) (u:usage info ip): pkg ip = Pkg 
+  info 
+  (salt ip u)
+  secret_len
   create_salt 
   coerce_salt
 
-let saltp2 (expu:usage) (ip:ipkg): pkg ip = Pkg 
-  (salt expu ip)
-  (fun _ -> 16ul) 
+let saltp2 (ip:ipkg) (u:usage info ip) : pkg ip = Pkg 
+  info 
+  (salt ip u)
+  secret_len
   create_salt 
   coerce_salt
+
 
 /// HKDF.Extract(key=0, materials=k) idealized as a single-use PRF,
 /// possibly customized on the distribution of k.
 assume val extract0:
-  #expu: usage ->
+  #u: usage info ii ->
   #i: id ->
-  k: psk expu ii i -> 
-  secret expu ii (Extract0 i)
+  #a: info ->
+  k: psk #ii #u i a -> 
+  secret ii u (Extract0 i) a
 
 /// HKDF.Extract(key=s, materials=dh_secret) idealized as 2-bit
 /// (KEF-ODH, KEF-Salt game); we will need separate calls for clients
 /// and servers.
 assume val extract1:
-  #expu: usage -> 
+  #u: usage info ii -> 
   #i: id ->
-  s: salt expu ii i ->
+  #a: info -> 
+  s: salt ii u i a ->
   materials: id_dhe -> 
-  secret expu ii (Extract1 i materials)
+  secret ii u (Extract1 i materials) a
 
 /// HKDF.Extract(key=s, materials=0) idealized as a single-use PRF.
 assume val extract2: 
-  #expu: usage ->
+  #u: usage info ii ->
   #i: id ->
-  s: salt expu ii i -> 
-  secret expu ii (Extract2 i)
-
-
-/// module Raw
-/// a default functionality (no idealization);
-/// for modelling, we could also provide a "leak" function
-type raw  (#ip: ipkg) (i: Idx?.t ip) = list nat 
-let create_raw (#ip: ipkg) (i: Idx?.t ip): raw  i  = [1;2;3] // should sample instead
-let coerce_raw (#ip: ipkg) (i: Idx?.t ip) _ : raw i  = [1;2;3] // should sample instead
-let rp (ip:ipkg): pkg ip = Pkg raw (fun _ -> 16ul) create_raw coerce_raw
-
-
-/// module AEAD
-/// Some other sample functionality,
-/// with a different concrete key representation
-assume new type key (#ip: ipkg) (i: Idx?.t ip) // abstraction required for indexing
-assume val coerce_key: #ip: ipkg -> i: Idx?.t ip -> lbytes 20ul -> key i 
-assume val dummy: lbytes 20ul
-let create_key (#ip: ipkg) (i: Idx?.t ip) : key i = coerce_key i dummy (* strange bug with coerce *)
-let mp (ip:ipkg): pkg ip = Pkg key (fun _ -> 20ul) create_key coerce_key
-
-val encrypt: #ip:ipkg -> #i:Idx?.t ip -> k: key i -> nat -> nat 
-let encrypt #ip #i k v = v + 1
+  #a: info ->
+  s: salt ii u i a -> 
+  secret ii u (Extract2 i) a
 
 
 /// module KeySchedule
@@ -240,36 +307,45 @@ let encrypt #ip #i k v = v + 1
 
 // not sure how to enforce label restrictions, e.g.
 // val u_traffic: s:string { s = "ClientKey" \/ s = "ServerKey"} -> ip:ipkg -> pkg ip
- 
-let u_traffic = function 
-  | "ClientKey" | "ServerKey" -> mp
-  | _ -> rp 
+
+let some_keylen: keylen = 32ul
+
+let u_default:  p:pkg ii & (ctx:info -> p.use)  = (| rp ii, (fun (a:info) -> some_keylen) |)
+
+let u_traffic: usage info ii = function 
+  | "ClientKey" | "ServerKey" -> (| mp ii , (fun (a:info) -> a.aea) |)
+  | _ -> u_default
 
 // #set-options "--print_universes --print_implicits"
 
-let rec u_master_secret (n:nat ): Tot usage (decreases (%[n; 0])) = function 
-  | "traffic" -> pp u_traffic 
-  | "resumption" -> if n > 0 then pskp (u_early_secret (n-1)) else rp 
-  | _ -> rp
-and u_handshake_secret (n:nat): Tot usage (decreases (%[n; 1])) = function 
-  | "traffic" -> pp u_traffic 
-  | "salt" -> saltp2 (u_master_secret n) 
-  | _ -> rp
-and u_early_secret (n:nat): Tot usage (decreases (%[n;2])) = function
-  | "traffic" -> pp u_traffic
-  | "salt" -> saltp1 (u_handshake_secret n) 
-  | _ -> rp 
+let rec u_master_secret (n:nat ): Tot (usage info ii) (decreases (%[n; 0])) = function 
+  | "traffic" -> (| pp ii u_traffic, (fun a -> a) |)
+  | "resumption" -> if n > 0 then (| pskp ii (u_early_secret (n-1)), (fun (a:info) -> a)|) else (| rp ii, (fun (a:info) -> some_keylen) |)
+  | _ -> u_default
+and u_handshake_secret (n:nat): Tot (usage info ii) (decreases (%[n; 1])) = function 
+  | "traffic" -> (| pp ii u_traffic , (fun (a:info) -> a) |)
+  | "salt" -> (| saltp2 ii (u_master_secret n), (fun (a:info) -> a) |)
+  | _ -> u_default
+and u_early_secret (n:nat): Tot (usage info ii) (decreases (%[n;2])) = function
+  | "traffic" -> (| pp ii u_traffic, (fun (a:info) -> a) |)
+  | "salt" -> (| saltp1 ii (u_handshake_secret n), (fun (a:info) -> a) |)
+  | _ -> u_default
 
 /// Tot required... can we live with this integer indexing?
 /// One cheap trick is to store a PSK only when it enables resumption.
 
 /// Testing normalization works for a parametric depth
 assume val depth:  n:nat {n > 1} 
-let u: usage = u_early_secret depth 
+let u: usage info ii = u_early_secret depth 
 let i0 = Extract0 (Preshared 0)
 
 /// Usability?
-let psk0: psk u ii (Preshared 0) = create_psk  (Preshared 0)
+
+let a = { ha=SHA1; aea=AES_GCM256 }
+
+let psk0: psk #ii #u (Preshared 0) a = create_psk  (Preshared 0)
+
+(* 
 let early_secret: secret u ii i0 = extract0 psk0
 
 val early_traffic: secret u_traffic ii (Derived i0 "traffic") 
@@ -339,3 +415,6 @@ let next_early_secret = extract0 rsk
 //
 // let k1' = derive k0 "secret" 
 // let k2' = derive #(u 22)  k1'  "aead"  // the type is not normalized; the key is not usable.
+
+
+TMP*)
